src/program_proof/mvcc/mvcc_inv.v
@@ -6,7 +6,6 @@ Definition mvccN := nroot.
 Definition mvccNTuple := nroot .@ "tuple".
 Definition mvccNGC := nroot .@ "gc".
 Definition mvccNSST := nroot .@ "sst".
-Definition mvccNDB := nroot .@ "db".
 
 Section def.
 Context `{!heapGS Σ, !mvcc_ghostG Σ}.
@@ -111,41 +110,6 @@ Proof. unfold mvcc_inv_sst_def. apply _. Defined.
 
 Definition mvcc_inv_sst γ p : iProp Σ :=
   inv mvccNSST (mvcc_inv_sst_def γ p).
-
-Definition frac_ptsto (γ : mvcc_names) (q : Qp) (k : u64) (v : dbval) : iProp Σ.
-Admitted.
-
-Lemma frac_ptsto_agree {γ q1 q2 k v1 v2} :
-  frac_ptsto γ q1 k v1 -∗
-  frac_ptsto γ q2 k v2 -∗
-  ⌜v1 = v2⌝.
-Admitted.
-
-Lemma frac_ptsto_update {γ q1 q2 k v1 v2} v :
-  (q1 + q2 = 1)%Qp ->
-  frac_ptsto γ q1 k v1 -∗
-  frac_ptsto γ q2 k v2 ==∗
-  frac_ptsto γ q1 k v ∗ frac_ptsto γ q2 k v.
-Admitted.
-
-Instance mvcc_frac_ptsto γ q k v :
-  Timeless (frac_ptsto γ q k v).
-Admitted.
-
-Definition mvcc_inv_db_def γ : iProp Σ :=
-  ∃ (m : dbmap) (v : dbval),
-    "Hdbpts" ∷ dbmap_ptstos γ m ∗
-    "Hptsto" ∷ frac_ptsto γ (1 / 2)%Qp (U64 0) v ∗
-    "%Hval"  ∷ ⌜m !! (U64 0) = Some v⌝ ∗
-    "%Hdom"  ∷ ⌜dom m = keys_all⌝.
-
-#[global]
-Instance mvcc_inv_db_timeless γ :
-  Timeless (mvcc_inv_db_def γ).
-Proof. unfold mvcc_inv_db_def. apply _. Defined.
-
-Definition mvcc_inv_db γ : iProp Σ :=
-  inv mvccNDB (mvcc_inv_db_def γ).
 
 End def.
 
@@ -400,10 +364,10 @@ Theorem per_key_inv_dbmap_ptstos_update {γ tmods tid} ts {m : dbmap} {past} r m
   dom mods ⊆ dom r ->
   (tid < ts)%nat ->
   dbmap_auth γ m -∗
-  dbmap_ptstos γ r -∗
+  dbmap_ptstos γ 1 r -∗
   ([∗ set] k ∈ keys_all, per_key_inv_def γ k tmods tid m past) ==∗
   dbmap_auth γ (mods ∪ m) ∗
-  dbmap_ptstos γ (mods ∪ r) ∗
+  dbmap_ptstos γ 1 (mods ∪ r) ∗
   ([∗ set] k ∈ keys_all, per_key_inv_def γ k ({[ (tid, mods) ]} ∪ tmods) ts (mods ∪ m) past).
 Proof using heapGS0 mvcc_ghostG0 Σ.
   iIntros "%Hdom %Htid Hdb Hdbpts Hkeys".
